KamiCorrectness.v
@@ -21,6 +21,7 @@ Definition EffectlessRelation {k: Kind} (R: RegsT -> RegsT -> Prop) (a_i a_s: Ac
 
 Definition ActionWb {k} myRegs (act: ActionT type k): Prop :=
   forall o reads upds calls ret,
+    NoDup (map fst o) ->
     SemAction o act reads upds calls ret ->
     ((exists o', SubList o' o /\ SubList reads o'
                  /\ getKindAttr o' = myRegs
